src/Std/Data/DHashMap/RawLemmas.lean
@@ -48,7 +48,8 @@ private meta def baseNames : Array Name :=
     ``getKey?_eq, ``getKey_eq, ``getKey!_eq, ``getKeyD_eq,
     ``insertMany_eq, ``Const.insertMany_eq, ``Const.insertManyIfNewUnit_eq,
     ``ofList_eq, ``Const.ofList_eq, ``Const.unitOfList_eq,
-    ``alter_eq, ``Const.alter_eq, ``modify_eq, ``Const.modify_eq, ``union_eq, ``inter_eq]
+    ``alter_eq, ``Const.alter_eq, ``modify_eq, ``Const.modify_eq, ``union_eq, ``inter_eq,
+    ``fst_partition_eq, ``snd_partition_eq]
 
 /-- Internal implementation detail of the hash map -/
 scoped syntax "simp_to_raw" ("using" term)? : tactic
@@ -5545,327 +5546,34 @@ end Const
 
 end map
 
-theorem size_partition [EquivBEq α] [LawfulHashable α] {p : (a : α) → β a → Bool} (h : m.WF) :
+theorem size_fst_partition_add_size_snd_partition_eq_size [EquivBEq α] [LawfulHashable α]
+    {p : (a : α) → β a → Bool} (h : m.WF) :
     (m.partition p).1.size + (m.partition p).2.size = m.size := by
-  simp only [partition, fold_eq_foldl_toList h]
-  let f : Raw α β × Raw α β → List ((a : α) × β a) → Raw α β × Raw α β :=
-    fun pair l => List.foldl (fun a b => if p b.1 b.2 = true
-      then (a.1.insert b.1 b.2, a.2) else (a.1, a.2.insert b.1 b.2)) pair l
-  suffices ∀ (l : List ((a : α) × β a)) (m₁ m₂ : Raw α β) (h₁ : m₁.WF) (h₂ : m₂.WF)
-      (h₃ : ∀ x ∈ l, ¬ x.1 ∈ m₁  ∧ ¬ x.1 ∈ m₂)
-      (h₄ : l.Pairwise (fun a b => (a.1 == b.1) = false)),
-      (f (m₁, m₂) l).1.size + (f (m₁, m₂) l).2.size = l.length + m₁.size + m₂.size by
-    have := this m.toList ∅ ∅ WF.empty WF.empty (by simp) (distinct_keys_toList h)
-    simp only [length_toList h, size_empty, Nat.add_zero, f] at this
-    apply this
-  intro l
-  induction l with
-  | nil => simp [f]
-  | cons hd tl ih =>
-    intro m₁ m₂ h₁ h₂ h₃ h₄
-    simp only [List.foldl_cons, List.length_cons, f]
-    by_cases h : p hd.1 hd.2 = true
-    · simp only [h, ↓reduceIte]
-      rw [ih _ _ (WF.insert h₁) h₂]
-      · rw [size_insert h₁]
-        simp only [(h₃ hd (by simp)), ↓reduceIte, Nat.add_right_cancel_iff]
-        omega
-      · intro x hx
-        simp only [List.pairwise_cons] at h₄
-        simp [h₁, h₄.1 x hx, h₃ x (by simp [hx])]
-      · apply List.Pairwise.of_cons h₄
-    · simp only [h, Bool.false_eq_true, ↓reduceIte]
-      rw [ih _ _ h₁ (WF.insert h₂)]
-      · rw [size_insert h₂]
-        simp only [(h₃ hd (by simp)), ↓reduceIte]
-        omega
-      · intro x hx
-        simp only [List.pairwise_cons] at h₄
-        simp [h₂, h₄.1 x hx, h₃ x (by simp [hx])]
-      · apply List.Pairwise.of_cons h₄
+  simp_to_raw using Raw₀.size_partition
 
-theorem partition_not_fst_eq_partition_snd [EquivBEq α] [LawfulHashable α]
+@[simp]
+theorem fst_partition_not_eq_partition_snd [EquivBEq α] [LawfulHashable α]
     {p : (a : α) → β a → Bool} (h : m.WF) :
     (m.partition (fun a b => ! p a b)).fst = (m.partition p).snd := by
-  simp only [partition, Bool.not_eq_eq_eq_not, Bool.not_true, fold_eq_foldl_toList h]
-  let f : Raw α β × Raw α β → List ((a : α) × β a) → Raw α β × Raw α β :=
-    fun pair l => List.foldl (fun a b => if p b.1 b.2 = true
-      then (a.1.insert b.1 b.2, a.2) else (a.1, a.2.insert b.1 b.2)) pair l
-  let f' : Raw α β × Raw α β → List ((a : α) × β a) → Raw α β × Raw α β :=
-    fun pair l => List.foldl (fun a b => if p b.1 b.2 = false
-      then (a.1.insert b.1 b.2, a.2) else (a.1, a.2.insert b.1 b.2)) pair l
-  suffices ∀ (l : List ((a : α) × β a)) (m₁ m₂ : Raw α β) (h₁ : m₁.WF) (h₂ : m₂.WF),
-    (f' (m₁, m₂) l).fst = (f (m₂, m₁) l).snd from this _ _ _ WF.empty WF.empty
-  intro l
-  induction l with
-  | nil => simp [f, f']
-  | cons hd tl ih =>
-    intro m₁ m₂ h₁ h₂
-    simp only [List.foldl_cons, f', f]
-    by_cases hhd : p hd.fst hd.snd = true
-    · simp only [hhd, Bool.true_eq_false, ↓reduceIte]
-      rw [ih _ _ h₁ (WF.insert h₂)]
-    · simp only [hhd, ↓reduceIte, Bool.false_eq_true]
-      rw [ih _ _ (WF.insert h₁) h₂]
+  simp_to_raw
+  rw [Raw₀.fst_partition_not_eq_snd_partition]
 
-theorem wf_partition_fst [EquivBEq α] [LawfulHashable α] (h : m.WF) {p : (a : α) → β a → Bool} :
-    (m.partition p).1.WF := by
-  simp only [partition, fold_eq_foldl_toList h]
-  let f : Raw α β × Raw α β → List ((a : α) × β a) → Raw α β × Raw α β :=
-    fun pair l => List.foldl (fun a b => if p b.1 b.2 = true
-      then (a.1.insert b.1 b.2, a.2) else (a.1, a.2.insert b.1 b.2)) pair l
-  suffices ∀ (l : List ((a : α) × β a)) (m₁ m₂ : Raw α β) (h₁ : m₁.WF) (h₂ : m₂.WF),
-    (f (m₁, m₂) l).1.WF from this _ _ _ WF.empty WF.empty
-  intro l
-  induction l with
-  | nil =>
-    simp only [List.foldl_nil, f]
-    intro m₁ _ h₁ _
-    apply h₁
-  | cons hd tl ih =>
-    intro m₁ m₂ h₁ h₂
-    simp only [List.foldl_cons, f]
-    by_cases hhd : p hd.fst hd.snd = true
-    · simp only [hhd, ↓reduceIte]
-      apply ih _ _ (WF.insert h₁) h₂
-    · simp only [hhd, Bool.false_eq_true, ↓reduceIte]
-      apply ih _ _ h₁ (WF.insert h₂)
+@[simp]
+theorem snd_partition_not_eq_partition_fst [EquivBEq α] [LawfulHashable α]
+    {p : (a : α) → β a → Bool} (h : m.WF) :
+    (m.partition (fun a b => ! p a b)).snd = (m.partition p).fst := by
+  simp_to_raw
+  rw [Raw₀.snd_partition_not_eq_fst_partition]
 
-section Perm
-
-variable {α : Type u}
-
-theorem List.Perm.of_nodup_of_nodup_of_forall_mem_iff_mem {α : Type u} (l₁ l₂ : List α)
-    (h₁ : l₁.Nodup) (h₂ : l₂.Nodup) (h₃ : ∀ (a : α), a ∈ l₁ ↔ a ∈ l₂) :
-    l₁.Perm l₂ := by
-  induction l₁ generalizing l₂ with
-  | nil =>
-    cases l₂ with
-    | nil => simp
-    | cons hd tl =>
-      specialize h₃ hd
-      simp at h₃
-  | cons hd tl ih =>
-    have hd_mem : hd ∈ l₂ := (h₃ hd).mp (by simp)
-    rw [List.mem_iff_append] at hd_mem
-    rcases hd_mem with ⟨pre, post, h⟩
-    rw [h]
-    apply List.Perm.trans ?_ List.perm_middle.symm
-    apply List.Perm.cons
-    have nodup_pre_post : (pre ++ post).Nodup := by
-      rw [h] at h₂
-      have := List.Perm.nodup List.perm_middle h₂
-      simp only [List.nodup_cons, List.mem_append, not_or] at this
-      apply this.2
-    apply ih
-    · simp only [List.nodup_cons] at h₁
-      apply h₁.2
-    · apply nodup_pre_post
-    · simp only [List.mem_append]
-      intro x
-      constructor
-      · intro hx
-        specialize h₃ x
-        simp only [List.mem_cons, hx, or_true, h, List.mem_append, true_iff] at h₃
-        simp only [h] at h₂
-        cases h₃ with
-        | inl h => apply Or.inl h
-        | inr h =>
-          cases h with
-          | inl h =>
-            rw [h] at hx
-            simp only [List.nodup_cons] at h₁
-            simp [hx] at h₁
-          | inr h =>
-            apply Or.inr h
-      · intro h'
-        simp only [h, List.nodup_append, List.nodup_cons, List.mem_cons, ne_eq,
-          forall_eq_or_imp] at h₂
-        rw [h] at h₃
-        specialize h₃ x
-        simp only [List.mem_cons, List.mem_append] at h₃
-        cases h' with
-        | inl h' =>
-          simp only [h', true_or, iff_true] at h₃
-          cases h₃ with
-          | inl h₃ =>
-            have := (h₂.2.2 x h').1
-            contradiction
-          | inr h₃ =>
-            apply h₃
-        | inr h' =>
-          simp only [h', or_true, iff_true] at h₃
-          cases h₃ with
-          | inl h₃ =>
-            have := (h₂.2.1.1)
-            simp [← h₃, h'] at this
-          | inr h₃ =>
-            apply h₃
-
-end Perm
-
-theorem mem_toList_insert [EquivBEq α] [LawfulHashable α] (h : m.WF) {k : α} {v : β k}
-    {x : (a : α) × β a} (h' : ¬ k ∈ m) :
-    x ∈ (m.insert k v).toList ↔ x ∈ m.toList ∨ x = ⟨k, v⟩ := by
-  have : containsₘ ⟨m, h.size_buckets_pos⟩ k = false := by
-    simp only [← contains_eq_containsₘ]
-    rw [mem_iff_contains] at h'
-    simp only [contains, h.size_buckets_pos, ↓reduceDIte, Bool.not_eq_true] at h'
-    apply h'
-  simp only [toList, insert, h.size_buckets_pos, ↓reduceDIte, insert_eq_insertₘ, insertₘ, this,
-    Bool.false_eq_true, ↓reduceIte, foldRev_cons, List.append_nil]
-  rw [List.Perm.mem_iff (toListModel_expandIfNecessary (consₘ ⟨m, h.size_buckets_pos⟩ k v))]
-  rw [List.Perm.mem_iff (toListModel_consₘ ⟨m, h.size_buckets_pos⟩ (Raw.WF.out h) k v)]
-  simp [Or.comm]
-
-theorem mem_toList_fst_partition [EquivBEq α] [LawfulHashable α] (h : m.WF)
-    {p : (a : α) → β a → Bool} (x : (a : α) × β a) :
-    x ∈ (m.partition p).1.toList ↔ x ∈ m.toList ∧ p x.1 x.2 = true := by
-  simp only [partition, fold_eq_foldl_toList h]
-  let f : Raw α β × Raw α β → List ((a : α) × β a) → Raw α β × Raw α β :=
-    fun pair l => List.foldl (fun a b => if p b.1 b.2 = true
-      then (a.1.insert b.1 b.2, a.2) else (a.1, a.2.insert b.1 b.2)) pair l
-  suffices ∀ (l : List ((a : α) × β a)) (m₁ m₂ : Raw α β) (h₁ : m₁.WF) (h₂ : m₂.WF)
-    (h₃ : ∀ x ∈ l, ¬ x.1 ∈ m₁)
-    (h₄ : l.Pairwise (fun a b => (a.1 == b.1) = false)),
-      x ∈ (f (m₁, m₂) l).1.toList ↔ (x ∈ l ∧ p x.1 x.2 = true) ∨ x ∈ m₁.toList by
-    specialize this m.toList ∅ ∅ WF.empty WF.empty (by simp) (distinct_keys_toList h)
-    rw [this]
-    simp
-  intro l
-  induction l with
-  | nil =>
-    simp [f]
-  | cons hd tl ih =>
-    intro m₁ m₂ h₁ h₂ h₃ h₄
-    simp only [List.foldl_cons, List.mem_cons, f]
-    by_cases hhd : p hd.1 hd.2
-    · simp only [hhd, ↓reduceIte]
-      rw [ih _ _ (WF.insert h₁) h₂]
-      · rw [mem_toList_insert h₁ (h₃ hd (by simp))]
-        constructor
-        · intro h
-          cases h with
-          | inl h =>
-            apply Or.inl (And.intro (Or.inr h.1) h.2)
-          | inr h =>
-            cases h with
-            | inl h =>
-              apply Or.inr h
-            | inr h =>
-              rw [h]
-              simp [hhd]
-        · intro h
-          cases h with
-          | inl h =>
-            rcases h with ⟨h, h'⟩
-            cases h with
-            | inl h =>
-              rw [h]
-              simp [hhd]
-            | inr h =>
-              simp [h, h']
-          | inr h =>
-            simp [h]
-      · intro x hx
-        simp only [mem_insert h₁, not_or, Bool.not_eq_true]
-        constructor
-        · simp only [List.pairwise_cons] at h₄
-          apply h₄.1 x hx
-        · apply h₃ x (by simp [hx])
-      · simp only [List.pairwise_cons] at h₄
-        apply h₄.2
-    · simp only [hhd, Bool.false_eq_true, ↓reduceIte]
-      rw [ih _ _ h₁ (WF.insert h₂)]
-      · constructor
-        · intro h
-          cases h with
-          | inl h =>
-            apply Or.inl (And.intro (Or.inr h.1) h.2)
-          | inr h =>
-            apply Or.inr h
-        · intro h
-          cases h with
-          | inl h =>
-            rcases h with ⟨h, h'⟩
-            cases h with
-            | inl h =>
-              rw [h] at h'
-              contradiction
-            | inr h =>
-              simp [h, h']
-          | inr  h =>
-            simp [h]
-      · simp only [List.mem_cons, forall_eq_or_imp] at h₃
-        apply h₃.2
-      · simp only [List.pairwise_cons] at h₄
-        apply h₄.2
-
-theorem nodup_toList [EquivBEq α] [LawfulHashable α] (h : m.WF) : m.toList.Nodup := by
-  simp only [List.Nodup, ne_eq]
-  suffices ∀ (l : List ((a :α) × β a)) (h₁ : List.Pairwise (fun a b => (a.1 == b.1) = false) l),
-    List.Pairwise (fun a b => a ≠ b) l from this m.toList (distinct_keys_toList h)
-  intro l
-  induction l with
-  | nil => simp
-  | cons hd tl ih =>
-    simp
-    intro h₁ h₂
-    refine And.intro ?_ (ih h₂)
-    intro a ha
-    false_or_by_contra
-    rename_i h'
-    specialize h₁ a ha
-    simp [h'] at h₁
-
-theorem List.nodup_filter_of_nodup {α : Type u} {l : List α} (h : l.Nodup) {p : α → Bool} :
-    (l.filter p).Nodup := by
-  induction l with
-  | nil => simp
-  | cons hd tl ih =>
-    simp only [List.nodup_cons, List.filter] at h ⊢
-    split <;> simp [h, ih]
-
-theorem partition_fst_equiv_filter [EquivBEq α] [LawfulHashable α]
+theorem fst_partition_equiv_filter [EquivBEq α] [LawfulHashable α]
     {p : (a : α) → β a → Bool} (h : m.WF)  :
     (m.partition p).fst ~m m.filter p := by
-  apply Equiv.of_toList_perm
-  apply List.Perm.trans _ (toList_filter h).symm
-  apply List.Perm.of_nodup_of_nodup_of_forall_mem_iff_mem
-  · apply nodup_toList
-    apply wf_partition_fst h
-  · apply List.nodup_filter_of_nodup (nodup_toList h)
-  · intro a
-    simp [mem_toList_fst_partition h]
+  simp_to_raw using Raw₀.fst_partition_equiv_filter
 
-theorem getKey?_partition_fst [LawfulBEq α]
-    {p : (a : α) → β a → Bool} (h : m.WF) {k : α} :
-  (m.partition p).1.getKey? k = (m.getKey? k).pfilter (fun x h' =>
-    p x (m.get x (mem_of_getKey?_eq_some h h'))) := by
-  rw [← getKey?_filter h]
-  apply Equiv.getKey?_eq (wf_partition_fst h) (WF.filter h)
-  apply partition_fst_equiv_filter h
-
-theorem getKey?_partition_snd [LawfulBEq α]
-    {p : (a : α) → β a → Bool} (h : m.WF) {k : α} :
-  (m.partition p).2.getKey? k = (m.getKey? k).pfilter (fun x h' =>
-    ! p x (m.get x (mem_of_getKey?_eq_some h h'))) := by
-  rw [← partition_not_fst_eq_partition_snd h, ← getKey?_filter h (f := fun a b => ! p a b)]
-  apply Equiv.getKey?_eq (wf_partition_fst h) (WF.filter h)
-  apply partition_fst_equiv_filter h
-
-theorem size_partition_fst_le_size [EquivBEq α] [LawfulHashable α]
-    {p : (a : α) → β a → Bool} (h : m.WF) :
-    (m.partition p).1.size ≤ m.size := by
-  rw [Equiv.size_eq (wf_partition_fst h) (WF.filter h) (partition_fst_equiv_filter h)]
-  apply size_filter_le_size h
-
-theorem size_partition_snd_le_size [EquivBEq α] [LawfulHashable α]
-    {p : (a : α) → β a → Bool} (h : m.WF) :
-    (m.partition p).2.size ≤ m.size := by
-  rw [← partition_not_fst_eq_partition_snd h]
-  rw [Equiv.size_eq (wf_partition_fst h) (WF.filter h) (partition_fst_equiv_filter h)]
-  apply size_filter_le_size h
+theorem snd_partition_equiv_filter_not [EquivBEq α] [LawfulHashable α]
+    {p : (a : α) → β a → Bool} (h : m.WF)  :
+    (m.partition p).snd ~m m.filter (fun a b => ! p a b) := by
+  simp_to_raw using Raw₀.snd_partition_equiv_filter_not
 
 attribute [simp] contains_eq_false_iff_not_mem
 end Raw
